RG theory is clean now

src/algebraic/algebraic_graph_theory.v
@@ -2,6 +2,7 @@ Require Import Setoid Morphisms.
 Require Import Coq.Sets.Ensembles.
 
 Require Import List.
+Import ListNotations.
 Require Import Coq.Sorting.Permutation.
 
 Require Import GraphVerification.src.util.NatSet.
@@ -12,103 +13,90 @@ Require Import GraphVerification.src.relational_graph_theory.
 Require Import GraphVerification.src.algebraic.algebraic_graph.
 Require Import GraphVerification.src.algebraic.algebraic_graph_to_RG.
 
+(* Stating and proving Lemmas and Theorems about AGs *)
 
+(* This is used to verify that the axioms on the algebra of AGs are consistent
+with the interpretation of the expressions in terms of RGs *)
+Ltac AG_axiom_proof_automation_via_RG :=
+    unfold AG_equiv; simpl; firstorder.
 
-
-
-Ltac AG_axiom_proof_automation_via_RG H H0 :=
-    unfold AG_equiv; intros; split; split; intros; simpl; simpl in H; repeat (destruct H || destruct H0); auto.
-
-(* These are the "8 axioms" originally proposed by  functional graphs with class *)
+(* These are the "8 axioms" originally proposed by functional graphs with class *)
 
 (* +++ is commutative and associative *)
 Theorem AG_Overlay_Commutative {A : Type} : forall (ag1 ag2 : AG A), ag1 +++ ag2 A== ag2 +++ ag1.
 Proof.
-    AG_axiom_proof_automation_via_RG H H0.
+    AG_axiom_proof_automation_via_RG.
 Qed.
 
 Theorem AG_Overlay_Associative {A : Type} : forall (ag1 ag2 ag3 : AG A), ag1 +++ (ag2 +++ ag3) A== (ag1 +++ ag2) +++ ag3.
 Proof.
-    AG_axiom_proof_automation_via_RG H H0.
+    AG_axiom_proof_automation_via_RG.
 Qed.
 
 (* (G, ***, e) is a monoid *)
 Theorem AG_Empty_Connect_L_Identity {A : Type} : forall (ag : AG A), Empty *** ag A== ag.
 Proof.
-    AG_axiom_proof_automation_via_RG H H0.
+    AG_axiom_proof_automation_via_RG.
 Qed.
 
 Theorem AG_Empty_Connect_R_Identity {A : Type} : forall (ag : AG A), ag *** Empty A== ag.
 Proof.
-    AG_axiom_proof_automation_via_RG H H0.
+    AG_axiom_proof_automation_via_RG.
 Qed.
 
 Theorem AG_Connect_Associative {A : Type} : forall (ag1 ag2 ag3 : AG A), ag1 *** (ag2 *** ag3) A== (ag1 *** ag2) *** ag3.
 Proof.
-    AG_axiom_proof_automation_via_RG H H0.
+    AG_axiom_proof_automation_via_RG.
 Qed.
 
 (* *** distributes over +++ *)
 Theorem AG_Connect_Overlay_L_Distributes {A : Type} : forall (ag1 ag2 ag3 : AG A), ag1 *** (ag2 +++ ag3) A== ag1 *** ag2 +++ ag1 *** ag3.
 Proof.
-    AG_axiom_proof_automation_via_RG H H0.
+    AG_axiom_proof_automation_via_RG.
 Qed.
 
 Theorem AG_Connect_Overlay_R_Distributes {A : Type} : forall (ag1 ag2 ag3 : AG A), (ag1 +++ ag2) *** ag3 A== ag1 *** ag3 +++ ag2 *** ag3.
 Proof.
-    AG_axiom_proof_automation_via_RG H H0.
+    AG_axiom_proof_automation_via_RG.
 Qed.
 
 (* Decomposition *)
 Theorem AG_Connect_Decomposition {A : Type} : forall (ag1 ag2 ag3 : AG A), ag1 *** ag2 *** ag3 A== ag1 *** ag2 +++ ag1 *** ag3 +++ ag2 *** ag3.
 Proof.
-    AG_axiom_proof_automation_via_RG H H0.
+    AG_axiom_proof_automation_via_RG.
 Qed.
 
 
 
-(* Show that AG_to_RG is are "complete" and "sound"  *)
-(* TODO: this is not very urgent right now, but is possibly necessary for model-based specification *)
 
-(* Complete: *)
-(* Look at paper *)
-
-(* Sound: *)
-
-
-
-(* Section to make rewrite work with equiv_AG *)
+(* Section to make rewrite work with A== of Overlays and Connects *)
 (* This proof is based on R== being an equivalence relation *)
 Instance AG_Equivalence {A : Type} : Equivalence (@AG_equiv A).
 Proof.
     G_derived_equivalence_prover A unit (@AG_to_RG_unlE A).
 Qed.
-         
 
-Ltac Proper_proof_automation H1 := split; split; intros; simpl in *; destruct H1; firstorder.
-
+Ltac Proper_proof_automation := split; simpl in *; firstorder.
 
 Instance Proper_add {A : Type} : Proper ((@AG_equiv A) ==> AG_equiv ==> AG_equiv) Overlay.
 Proof.
-    Proper_proof_automation H1.
+    Proper_proof_automation.
 Qed.
-
 
 Instance Proper_mul {A : Type} : Proper ((@AG_equiv A) ==> AG_equiv ==> AG_equiv) Connect.
 Proof.
-    Proper_proof_automation H1.
+    Proper_proof_automation.
 Qed.
 
 
 
 
-(* Theorems that can be made based on the "8 axioms": 
-They can all be proven using "AG_axiom_proof_automation_via_RG", but I should find a way to do it using the axioms *)
-(* These proofs are heavily inspired by: http://async.org.uk/tech-reports/NCL-EEE-MICRO-TR-2014-191.pdf *)
+(* The following theorems are provable using the same automation as the 8 axioms,
+but this section aims to demonstrate their utility, by using only them.
+This has already been done in the Agda formalization by Andrey Mokhov *)
 
-
-(* This is a helper for Identity of + *)
-Lemma rdeco {A : Type}: forall (ag : AG A), ag +++ ag +++ Empty A== ag.
+(* This is a helper for multiple theorems *)
+Lemma _Overlay_preidempotence {A : Type}: forall (ag : AG A), ag +++ ag +++ Empty A== ag.
 Proof.
     intros.
     pose proof (AG_Connect_Decomposition ag Empty Empty).
@@ -125,7 +113,7 @@ Qed.
 Theorem AG_Empty_Overlay_R_Identity {A : Type}: forall (g : AG A), g +++ Empty A== g.
 Proof.
     intros.
-    rewrite <- rdeco.
+    rewrite <- _Overlay_preidempotence.
 
     rewrite <- AG_Overlay_Associative.
     rewrite (AG_Overlay_Associative Empty (g +++ Empty)). 
@@ -133,24 +121,23 @@ Proof.
     rewrite <- AG_Overlay_Associative.
     rewrite <- AG_Overlay_Associative.
 
-    rewrite (rdeco).
-    rewrite (rdeco).
+    rewrite _Overlay_preidempotence.
+    rewrite _Overlay_preidempotence.
     reflexivity.
 Qed.
 
 
-(* idempotence of + *)
+(* Idempotence of + *)
 Theorem AG_Overlay_Idempotence {A : Type}: forall (ag : AG A), ag +++ ag A== ag.
 Proof.
     intros.
-    pose proof rdeco ag.
+    pose proof _Overlay_preidempotence ag.
     rewrite AG_Empty_Overlay_R_Identity in H.
-    auto.
+    assumption.
 Qed.
 
 
-
-(* Absorption (proof is mine) *)
+(* Absorption *)
 Theorem AG_Absorption {A : Type}: forall (ag1 ag2 : AG A), ag1 *** ag2 +++ ag1 +++ ag2 A== ag1 *** ag2.
 Proof.
     intros. pose proof AG_Connect_Decomposition ag1 ag2 Empty.
@@ -159,11 +146,11 @@ Proof.
     rewrite AG_Empty_Connect_R_Identity in H.
     rewrite AG_Empty_Connect_R_Identity in H.
     symmetry in H.
-    auto.
+    assumption.
 Qed.
 
 
-(* Saturation (proof is mine) *)
+(* Saturation *)
 Theorem AG_Saturation {A : Type}: forall (ag : AG A), ag *** ag *** ag A== ag *** ag.
 Proof.
     intros.
@@ -192,171 +179,10 @@ Qed.
 
 
 
+(* Start Proving properties on AG_BFS *)
 
 
-
-
-
-
-(* Here, I start proving things about BFS *)
-
-
-
-Lemma if_result_same : forall (A : Type) (b : bool) (x : A), 
-    (if b then x else x) = x.
-Proof.
-    intros.
-    destruct b.
-    - reflexivity.
-    - reflexivity.
-Qed.
-
-Lemma NatSet_intersection_singleton : forall (s : NatSet.t) (x : nat),
-NatSet.mem x s = true -> NatSet.inter s (NatSet.singleton x) = NatSet.singleton x.
-Proof.
-Admitted.
-
-
-
-Lemma NatList_filterOutOf_makes_subset : forall (s : NatSet.t) (l : list nat),
-    incl (NatList_filterOutOf s l) l.
-Proof.
-    unfold incl. intros. unfold NatList_filterOutOf in H. apply filter_In in H. firstorder.
-Qed.
-
-
-
-Lemma NatList_filterOutOf_splits_In : forall (s : NatSet.t) (l : list nat) x,
-    In x l -> In x (NatSet.elements s) \/ In x (NatList_filterOutOf s l).
-Proof.
-    intros. induction l.
-    - simpl in H. firstorder.
-    - simpl in H. destruct H.
-        + subst. simpl. destruct (negb (NatSet.mem x s)) eqn:mem.
-            -- right. firstorder.
-            -- left. apply Bool.negb_false_iff in mem. apply NatSet.mem_spec in mem. apply NatSet.elements_spec1 in mem.
-                apply SetoidList.InA_alt in mem. destruct mem. destruct H. subst. assumption.
-        + specialize (IHl H). destruct IHl.
-            -- left.  assumption.
-            -- right. simpl. destruct (negb (NatSet.mem a s)).
-                ++ simpl. right. assumption.
-                ++ assumption.
-Qed.
-
-
-
- 
-
-
-
-Lemma consolidation_fold_right_preserves_nodes : forall (l : list (NatSet.t)) y,
-    (exists x, In x l /\ NatSet.In y x) <-> (In y (fold_right (fun (next : NatSet.t) (acc : list nat) => NatSet.elements next ++ NatList_filterOutOf next acc) nil l)) .
-Proof.
-    intros. induction l.
-    - simpl. firstorder.
-    - split; intros.
-        + destruct H. simpl in H. destruct H. destruct H.
-            -- subst. simpl. apply in_or_app. left. apply NatSet.elements_spec1 in H0.
-                apply SetoidList.InA_alt in H0. destruct H0. destruct H. subst. assumption.
-            -- assert (exists x : NatSet.t, In x l /\ NatSet.In y x). { firstorder.
-            } destruct IHl. specialize (H2 H1).
-              simpl. apply in_or_app. apply NatList_filterOutOf_splits_In. assumption.
-        + simpl in H.  apply in_app_or in H.  destruct H.
-            -- exists a. split.
-                ++ simpl. auto.
-                ++ apply NatSet.elements_spec1. apply SetoidList.InA_alt. exists y. auto.
-            -- destruct IHl. apply NatList_filterOutOf_makes_subset in H. apply H1 in H. firstorder.
-Qed.
-
-Lemma NatSet_In_is_In_elements : forall (s : NatSet.t) (x : nat),
-    NatSet.In x s <-> In x (NatSet.elements s).
-Proof.
-    intros. split; intros.
-    - apply NatSet.elements_spec1 in H. apply SetoidList.InA_alt in H. destruct H. destruct H. subst. assumption.
-    - apply NatSet.elements_spec1. apply SetoidList.InA_alt. exists x. auto.
-Qed.
-
-
-Lemma In_AG_nodeSet_is_In_RG : forall (ag : AG nat) (x : nat),
-    NatSet.In x (AG_nodeSet ag) <-> (AG_to_RG_unlE ag).(RG_nodes) x.
-Proof.
-Admitted.
-
-
-Lemma _singleStep_returns_only_nodes : forall (ag : AG nat) (from : NatSet.t),
-    forall x, NatSet.In x (_singleStep from ag) -> (AG_to_RG_unlE ag).(RG_nodes) x.
-Proof.
-    intros. induction ag.
-    - simpl in H. apply NatSet_In_is_In_elements in H. simpl in H. destruct H.
-    - simpl in H. apply NatSet_In_is_In_elements in H. simpl in H. destruct H.
-    - simpl. simpl in H. apply NatSet.union_spec in H. destruct H.
-     + left. apply IHag1. assumption.
-     + right. apply IHag2. assumption.
-     
-    - simpl. simpl in H. apply NatSet.union_spec in H. destruct H. 
-        + apply NatSet.union_spec in H. destruct H.
-            -- left. apply IHag1. assumption.
-            -- right. apply IHag2. assumption.
-        + destruct (NatSet.is_empty (NatSet.inter (AG_nodeSet ag1) from)) eqn:split.
-            -- apply NatSet_In_is_In_elements in H. simpl in H. destruct H.
-            -- right. apply In_AG_nodeSet_is_In_RG. assumption.
-Qed.
-
-(* Tactic Notation "skip" := admit. *)
-
-
-Lemma _upToNStepsCap_returns_only_nodes : forall (ag : AG nat) (from s: NatSet.t) (n : nat) x y,
-    NatSet.Subset from (AG_nodeSet ag) ->
-    In x (_upToNStepsCap_rec from s ag n) -> NatSet.In y x -> (AG_to_RG_unlE ag).(RG_nodes) y.
-Proof.
-    intros. generalize dependent from. generalize dependent s. induction n.
-    - intros. simpl in H. contradiction.
-    - intros. simpl in H0. destruct H0.
-        + subst. apply In_AG_nodeSet_is_In_RG. unfold NatSet.Subset in H. apply H. assumption.
-        + destruct (NatSet.equal s (NatSet.union s (_singleStep from ag))).  
-            -- simpl in H0. contradiction.
-            -- specialize (IHn (NatSet.union s (_singleStep from ag))  (_singleStep from ag)).
-               apply IHn.
-               ++ unfold NatSet.Subset. intros.
-               apply _singleStep_returns_only_nodes in H2. apply In_AG_nodeSet_is_In_RG. assumption.
-               ++ assumption.
-Qed.
-
-
-            
-            
-Lemma _upToNStepsCapCaller_returns_only_nodes : forall (ag : AG nat) (from : NatSet.t) (n : nat) x y,
-    In x (_upToNStepsCap from ag n) -> NatSet.In y x -> (AG_to_RG_unlE ag).(RG_nodes) y.
-Proof.
-    intros.
-    pose proof _upToNStepsCap_returns_only_nodes.
-    specialize (H1 ag (NatSet.inter from (AG_nodeSet ag)) (NatSet.inter from (AG_nodeSet ag)) (S n) x).
-    apply H1.
-    - unfold NatSet.Subset. intros. apply NatSet.inter_spec in H2. destruct H2. assumption.
-    - unfold _upToNStepsCap in H. apply H.
-    - assumption.
-Qed.
-
-
-
-
-
-
-Theorem AG_BFS_returns_only_nodes : forall (nodes : list nat) (ag : AG nat),
-  forall x, In x (AG_BFS nodes ag) -> (AG_to_RG_unlE ag).(RG_nodes) x. 
-Proof.
-    intros. unfold AG_BFS in H. apply consolidation_fold_right_preserves_nodes in H.
-        destruct H. destruct H.
-        apply (_upToNStepsCapCaller_returns_only_nodes _ _ _ _ x) in H.
-        + assumption.
-        + assumption.
-Qed.
-
-
-
-
-
-(* https://plv.mpi-sws.org/c11comp/coq/extralib.html *)
+(* Some more basics about NoDup and disjointness: *)
 Definition disjoint {A : Type} (l1 l2 : list A) :=
   forall a, In a l1 /\ In a l2 -> False.  
 
@@ -365,14 +191,34 @@ Lemma nodup_app: forall (A: Type) (l1 l2: list A),
   NoDup (l1 ++ l2) <->
   NoDup l1 /\ NoDup l2 /\ disjoint l1 l2.
 Proof.
-Admitted.
+    intros. unfold disjoint. induction l1; simpl.
+    - firstorder. apply NoDup_nil.
+    - split; intros.
+        + inversion H. apply IHl1 in H3. destruct H3 as [H30 [H31 H32]].
+            split.
+            -- apply NoDup_cons.
+                ++ unfold not. intros. unfold not in H2. apply H2. apply in_or_app. firstorder.
+                ++ assumption.
+            -- split.
+                ++ assumption.
+                ++ subst. intros. unfold not in H2. apply H2.
+                    simpl in *. destruct H0. apply in_or_app. destruct H0.
+                    --- subst. auto.
+                    --- firstorder.
+        + destruct H. destruct H0. inversion H. apply NoDup_cons.
+            -- subst. unfold not. intros.
+                apply in_app_or in H2. apply (H1 a). firstorder.
+            -- apply IHl1. firstorder.
+Qed.
 
 
-Lemma NatList_filterOutOf_disjoint : forall (s : NatSet.t) (l : list nat),
-    disjoint (NatSet.elements s) (NatList_filterOutOf s l).
+
+(* Some Helper Lemmas on NatSets and their elements *)
+Lemma NatSet_In_is_In_elements : forall (x : Node) (s : NatSet.t),
+    NatSet.In x s <-> In x (NatSet.elements s).
 Proof.
-Admitted.
-
+    intros. rewrite <- NatSet.elements_spec1. rewrite SetoidList.InA_alt. firstorder. subst. auto.
+Qed.
 
 Lemma NoDup_NatSet_elements : forall (s : NatSet.t),
     NoDup (NatSet.elements s).
@@ -386,6 +232,43 @@ Qed.
 
 
 
+(* Helper Lemmas on NatList_filterOutOf: *)
+Lemma NatList_filterOutOf_makes_subset : forall (s : NatSet.t) (l : list nat),
+    incl (NatList_filterOutOf s l) l.
+Proof.
+    unfold incl. intros. unfold NatList_filterOutOf in H. apply filter_In in H. firstorder.
+Qed.
+
+
+Lemma NatList_filterOutOf_splits_In : forall (s : NatSet.t) (l : list nat) x,
+    In x l -> In x (NatSet.elements s) \/ In x (NatList_filterOutOf s l).
+Proof.
+    intros. induction l; simpl in *.
+    - destruct H.
+    - destruct H.
+        + subst. destruct (negb (NatSet.mem x s)) eqn:mem.
+            -- right. firstorder.
+            -- left. apply Bool.negb_false_iff in mem. apply NatSet.mem_spec in mem. apply NatSet_In_is_In_elements. auto.
+        + specialize (IHl H). destruct IHl.
+            -- left.  assumption.
+            -- right. simpl. destruct (negb (NatSet.mem a s)); firstorder.
+Qed.
+
+Lemma NatList_filterOutOf_disjoint : forall (s : NatSet.t) (l : list nat),
+    disjoint (NatSet.elements s) (NatList_filterOutOf s l).
+Proof.
+    unfold disjoint. intros. destruct H.
+    unfold NatList_filterOutOf in H0.
+
+    apply NatSet_In_is_In_elements in H.
+
+    induction l.
+    - firstorder.
+    - simpl in H0. apply IHl. destruct (negb (NatSet.mem a0 s)) eqn:isin.
+        + firstorder. subst. apply Bool.negb_true_iff in isin. apply NatSet.mem_spec in H. rewrite H in isin. discriminate isin.
+        + assumption.
+Qed.
+
 Lemma NoDup_fold_right_filterOutOf : forall (l : list (NatSet.t)),
     NoDup (fold_right (fun (next : NatSet.t) (acc : list nat) => NatSet.elements next ++ NatList_filterOutOf next acc) nil l).
 Proof.
@@ -398,10 +281,6 @@ Proof.
             -- apply NatList_filterOutOf_disjoint.
 Qed.
 
-
-
-
-
 Theorem AG_BFS_no_duplicates : forall (nodes : list nat) (ag : AG nat),
   NoDup (AG_BFS nodes ag).
 Proof.
@@ -410,51 +289,115 @@ Proof.
     apply NoDup_fold_right_filterOutOf.
 Qed.
 
-Theorem AG_BFS_path : forall (nodes : list nat) (ag : AG nat) x y,
-  In x nodes -> (In y (AG_BFS nodes ag) <-> RG_existsPath x y (AG_to_RG_unlE ag)).
+
+
+
+Lemma _consolidation_fold_right_preserves_nodes : forall (l : list (NatSet.t)) y,
+    (exists x, In x l /\ NatSet.In y x) <-> (In y (fold_right (fun next acc => NatSet.elements next ++ NatList_filterOutOf next acc) nil l)) .
+Proof. 
+    intros. induction l; simpl.
+    - firstorder.
+    - split; intros.
+        + destruct H. simpl in H. destruct H. destruct H.
+            -- subst. simpl. apply in_or_app. left. apply NatSet_In_is_In_elements. auto.
+            -- simpl. apply in_or_app. apply NatList_filterOutOf_splits_In. apply IHl. firstorder.
+        + apply in_app_or in H. destruct H.
+            -- exists a. rewrite NatSet_In_is_In_elements. auto.
+            -- destruct IHl. apply NatList_filterOutOf_makes_subset in H. apply H1 in H. firstorder.
+Qed.
+
+
+
+Lemma In_AG_nodeSet_is_In_RG : forall (ag : AG nat),
+    forall x, NatSet.In x (AG_nodeSet ag) <-> (AG_to_RG_unlE ag).(RG_nodes) x.
 Proof.
-  intros.
-Admitted.
-
-Import ListNotations.
-
-(* 
-Inductive Is_BFS_ordered {A : Type} : list A -> Prop :=
-  | Is_BFS_ordered_nil : Is_BFS_ordered []
-  | Is_BFS_ordered_cons : forall (a : A) (l : list A), Is_BFS_ordered l -> Is_BFS_ordered (a :: l). *)
+    intros. induction ag.
+    - simpl. apply SProps.MP.FM.empty_iff.
+    - simpl. rewrite NatSet.singleton_spec. firstorder.
+    (* firstorder works, but is just too slow here *)
+    - simpl. rewrite NatSet.union_spec. rewrite IHag1. rewrite IHag2. reflexivity.
+    - simpl. rewrite NatSet.union_spec. rewrite IHag1. rewrite IHag2. reflexivity.
+Qed.
 
 
-(* Is, in general the search ordered in some single step manner? *)
-Fixpoint Is_Search_ordered_helper {A B : Type} (l passed : list A) (rg : RG A B) : Prop :=
-  match l with
-  | [] => True
-  | x :: xs => RG_reachableInOneStep (fun x => In x passed) x rg /\ Is_Search_ordered_helper xs (x :: passed) rg
-  end.
-
-
-Fixpoint trim {A : Type} (l passed : list A) : list A :=
-  match l, passed with
-  | le::ls, pe::ps => trim ls ps
-  | ls, [] => ls
-  | _, _ => nil
-  end.
-
-Fixpoint doesMatch {A : Type} (l passed : list A) : Prop :=
-  match l, passed with
-  | le::ls, pe::ps => le = pe /\ doesMatch ls ps
-  | _, [] => True
-  | _, _ => False
-  end.
-
-Definition Is_Search_ordered {A B : Type} (l passed : list A) (rg : RG A B) : Prop :=
-   let trimmedL := trim l passed in
-   let didMatch := doesMatch l passed in
-   didMatch /\ Is_Search_ordered_helper trimmedL passed rg. 
-
-
-Theorem AG_BFS_search_order : forall (nodes : list nat) (ag : AG nat),
-    Is_Search_ordered (AG_BFS nodes ag) nodes (AG_to_RG_unlE ag).
+Lemma _singleStep_returns_only_nodes : forall (from : NatSet.t) (ag : AG nat),
+    forall x, NatSet.In x (_singleStep from ag) -> (AG_to_RG_unlE ag).(RG_nodes) x.
 Proof.
+    intros. induction ag; simpl in *.
+    - apply NatSet_In_is_In_elements in H. simpl in H. destruct H.
+    - apply NatSet_In_is_In_elements in H. simpl in H. destruct H.
+    - apply NatSet.union_spec in H. destruct H. 
+        + left. apply IHag1. assumption.
+        + right. apply IHag2. assumption.
+     
+    - apply NatSet.union_spec in H. destruct H. 
+        + apply NatSet.union_spec in H. destruct H.
+            -- left. apply IHag1. assumption.
+            -- right. apply IHag2. assumption.
+        + destruct (NatSet.is_empty (NatSet.inter (AG_nodeSet ag1) from)) eqn:split.
+            -- apply NatSet_In_is_In_elements in H. simpl in H. destruct H.
+            -- right. apply In_AG_nodeSet_is_In_RG. assumption.
+Qed.
+
+
+
+Lemma _upToNStepsCap_rec_returns_only_nodes : forall (from s: NatSet.t) (ag : AG nat) (n : nat),
+    forall x y, NatSet.Subset from (AG_nodeSet ag) ->
+    In x (_upToNStepsCap_rec from s ag n) -> NatSet.In y x -> (AG_to_RG_unlE ag).(RG_nodes) y.
+Proof.
+    intros. generalize dependent from. generalize dependent s. induction n; intros; simpl in *.
+    - contradiction.
+    - destruct H0.
+        + subst. apply In_AG_nodeSet_is_In_RG. unfold NatSet.Subset in H. apply H. assumption.
+        + destruct (NatSet.equal s (NatSet.union s (_singleStep from ag))).  
+            -- simpl in H0. contradiction.
+            -- specialize (IHn (NatSet.union s (_singleStep from ag)) (_singleStep from ag)).
+               apply IHn.
+               ++ unfold NatSet.Subset. intros.
+                    apply _singleStep_returns_only_nodes in H2. apply In_AG_nodeSet_is_In_RG. assumption.
+               ++ assumption.
+Qed.
+
+
+
+Lemma _upToNStepsCap_returns_only_nodes : forall (from : NatSet.t) (ag : AG nat) (n : nat),
+    forall x y, In x (_upToNStepsCap from ag n) -> NatSet.In y x -> (AG_to_RG_unlE ag).(RG_nodes) y.
+Proof.
+    intros.
+    pose proof _upToNStepsCap_rec_returns_only_nodes.
+    specialize (H1 (NatSet.inter from (AG_nodeSet ag)) (NatSet.inter from (AG_nodeSet ag)) ag (S n) x).
+    apply H1.
+    - unfold NatSet.Subset. intros. apply NatSet.inter_spec in H2. destruct H2. assumption.
+    - unfold _upToNStepsCap in H. apply H.
+    - assumption.
+Qed.
+
+
+
+
+Theorem AG_BFS_returns_only_nodes : forall (nodes : list nat) (ag : AG nat),
+    forall x, In x (AG_BFS nodes ag) -> (AG_to_RG_unlE ag).(RG_nodes) x. 
+Proof.
+    intros. unfold AG_BFS in H. apply _consolidation_fold_right_preserves_nodes in H.
+    destruct H. destruct H.
+    apply (_upToNStepsCap_returns_only_nodes _ _ _ _ x) in H; auto.
+Qed.
+
+
+
+
+
+
+
+
+
+
+
+Theorem AG_BFS_path : forall (nodes : list nat) (ag : AG nat),
+    forall x y, In x nodes ->
+    (In y (AG_BFS nodes ag) <-> RG_existsPath x y (AG_to_RG_unlE ag)).
+Proof.
+    intros.
 Admitted.
 
 
@@ -465,75 +408,98 @@ Admitted.
 (* Now, the specification of a BFS search order: *)
 
 
-
-
-
-Inductive sameDistance {A B : Type} (rg : RG A B) : Ensemble A -> Ensemble A -> A -> A -> Prop :=
-    | bothInStart (start1 start2 : Ensemble A) : forall (a1 a2 : A), start1 a1 -> start2 a2 -> sameDistance rg start1 start2 a1 a2
+Inductive sameDistance_rec {A B : Type} (rg : RG A B) : Ensemble A -> A -> Ensemble A -> A -> Prop :=
+    | bothInStart (start1 start2 : Ensemble A) : forall (a1 a2 : A), start1 a1 -> start2 a2 -> sameDistance_rec rg start1 a1 start2 a2
     | bothOneStep (start1 start2 : Ensemble A) : forall (a1 a2 : A),
-        sameDistance rg (fun x => RG_reachableInOneStep start1 x rg) (fun x => RG_reachableInOneStep start2 x rg) a1 a2
-        -> sameDistance rg start1 start2 a1 a2 
-. 
+        sameDistance_rec rg (fun x => RG_reachableInOneStep start1 x rg) a1 (fun x => RG_reachableInOneStep start2 x rg) a2
+        -> sameDistance_rec rg start1 a1 start2 a2. 
 
-Definition sameDistanceCaller {A B : Type} (rg : RG A B) (start : Ensemble A) (a1 a2 : A) : Prop :=
-    sameDistance rg start start a1 a2.
+Definition sameDistance {A B : Type} (start : Ensemble A) (a1 a2 : A) (rg : RG A B) : Prop :=
+    sameDistance_rec rg start a1 start a2.
 
-Lemma sameDistance_caller_test1 : sameDistanceCaller (AG_to_RG_unlE (1 *** 2 +++ 1 *** 3)) (fun x => NatSet.In x (NatSet.singleton 1)) 2 3.
+Lemma sameDistance_caller_test1 : sameDistance (fun x => x = 1) 2 3 (AG_to_RG_unlE (1 *** 2 +++ 1 *** 3)).
 Proof.
-    unfold sameDistanceCaller.
+    unfold sameDistance.
     apply bothOneStep.
     apply bothInStart.
-    - simpl. unfold RG_reachableInOneStep. exists 1, tt. firstorder. apply SProps.MP.FM.singleton_iff. reflexivity.
- 
-    - simpl. unfold RG_reachableInOneStep. exists 1, tt. firstorder. apply SProps.MP.FM.singleton_iff. reflexivity.
+    - simpl. unfold RG_reachableInOneStep. exists 1, tt. firstorder.
+    - simpl. unfold RG_reachableInOneStep. exists 1, tt. firstorder.
 Qed.
 
 
 (* Returns true, if the distance from a1 to start is one plus the distance from a2 to start *)
-Definition distanceSecondOneLower {A B : Type} (rg : RG A B) (start : Ensemble A) (a1 a2 : A) : Prop :=
-    sameDistance rg (fun x => RG_reachableInOneStep start x rg) start a1 a2.
+Definition distanceSecondOneLower {A B : Type} (start : Ensemble A) (a1 a2 : A) (rg : RG A B) : Prop :=
+    sameDistance_rec rg (fun x => RG_reachableInOneStep start x rg) a1 start a2.
 
     
-Lemma distanceSecondOneLower_test1 : distanceSecondOneLower (AG_to_RG_unlE (1 *** 2 +++ 1 *** 3 +++ 3 *** 4)) (fun x => NatSet.In x (NatSet.singleton 1)) 4 2.
+Lemma distanceSecondOneLower_test1 : distanceSecondOneLower (fun x => x = 1) 4 2 (AG_to_RG_unlE (1 *** 2 +++ 1 *** 3 +++ 3 *** 4)).
 Proof.
     unfold distanceSecondOneLower.
     apply bothOneStep.
     apply bothInStart.
-    - simpl. unfold RG_reachableInOneStep. exists 3, tt. firstorder. exists 1, tt. firstorder. apply SProps.MP.FM.singleton_iff. reflexivity. 
-    - simpl. unfold RG_reachableInOneStep. exists 1, tt. firstorder. apply SProps.MP.FM.singleton_iff. reflexivity.
+    - simpl. unfold RG_reachableInOneStep. exists 3, tt. firstorder. exists 1, tt. firstorder.
+    - simpl. unfold RG_reachableInOneStep. exists 1, tt. firstorder.
 Qed.
 
 
 
 
 
-Inductive revBFSOrder (start : NatSet.t) (ag : AG nat) : list nat -> Prop :=
-  | revBFSOrder_start (l : list nat) : Permutation (NatSet.elements start) l -> revBFSOrder start ag l
+Inductive revBFSOrder {B : Type} (start : NatSet.t) (rg : RG nat B) : list nat -> Prop :=
+  | revBFSOrder_start (l : list nat) : Permutation (NatSet.elements start) l -> revBFSOrder start rg l
 
   | revBFSOrder_same (noww next : nat) (l : list nat) :
-    sameDistanceCaller (AG_to_RG_unlE ag) (fun x => NatSet.In x start) noww next -> revBFSOrder start ag (next :: l) -> revBFSOrder start ag (noww :: next :: l)   
+    sameDistance (fun x => NatSet.In x start) noww next rg -> revBFSOrder start rg (next :: l) -> revBFSOrder start rg (noww :: next :: l)   
 
   | revBFSOrder_next (noww next : nat) (l : list nat) :
-    distanceSecondOneLower (AG_to_RG_unlE ag) (fun x => NatSet.In x start) noww next 
-    -> revBFSOrder start ag (next :: l) -> revBFSOrder start ag (noww :: next :: l).
+    distanceSecondOneLower  (fun x => NatSet.In x start) noww next rg 
+    -> revBFSOrder start rg (next :: l) -> revBFSOrder start rg (noww :: next :: l).
+
+Definition BFSOrder {B : Type} (startL result : list nat) (rg : RG nat B) :=
+    revBFSOrder (NatSet_fromList startL) rg (rev result).
 
 
-
-Lemma revBFSOrder_test1 : revBFSOrder (NatSet.singleton 1) (1 *** 2 +++ 3 *** 4) [1; 2; 3; 4].
+Theorem AG_BFS_order : forall (nodes : list nat) (ag : AG nat),
+    BFSOrder nodes (AG_BFS nodes ag) (AG_to_RG_unlE ag).
 Proof.
+    intros.
 Admitted.
 
 
 
+Lemma revBFSOrder_test1 : BFSOrder [1] (AG_BFS [1] (1 *** 2 +++ 1 *** 3 +++ 3 *** 4)) (AG_to_RG_unlE (1 *** 2 +++ 1 *** 3 +++ 3 *** 4)).
+Proof.
+    unfold BFSOrder. simpl.
+    apply revBFSOrder_next.
+    - unfold distanceSecondOneLower. apply bothOneStep. apply bothInStart.
+        + unfold RG_reachableInOneStep. simpl. exists 3, tt. firstorder. exists 1, tt. firstorder.
+            apply NatSet.singleton_spec. reflexivity.
+        + unfold RG_reachableInOneStep. simpl. exists 1, tt. firstorder.
+            apply NatSet.singleton_spec. reflexivity.
+
+    - apply revBFSOrder_same.
+        + unfold sameDistance. apply bothOneStep. apply bothInStart.
+            -- unfold RG_reachableInOneStep. simpl. exists 1, tt. firstorder.
+                apply NatSet.singleton_spec. reflexivity.
+            -- unfold RG_reachableInOneStep. simpl. exists 1, tt. firstorder.
+                apply NatSet.singleton_spec. reflexivity.
+        + apply revBFSOrder_next.
+            -- unfold distanceSecondOneLower. apply bothInStart.
+                ++ unfold RG_reachableInOneStep. simpl. exists 1, tt. firstorder.
+                    apply NatSet.singleton_spec. reflexivity.
+                ++ apply NatSet.singleton_spec. reflexivity.
+            -- apply revBFSOrder_start. apply perm_skip. apply perm_nil.
+Qed.
 
 
 
-(* Here some things about "Transpose:" *)
 
+
+
+(* AG_transpose relates to RG_transpose *)
 Theorem AG_transpose_is_RG : forall (ag : AG nat),
     AG_to_RG_unlE (transpose ag) R== RG_transpose (AG_to_RG_unlE ag). 
 Proof.
     intros. induction ag; simpl; firstorder.
 Qed.
     
-
